Semantic/Capybara/Denotation/Rebind.lean
@@ -176,23 +176,23 @@ def rebind_val_denot
     constructor
     · intro ⟨hwf_e, hwf_cs, cs', S0, t0, hr, hwf_cs', hR0_sub, hd⟩
       refine ⟨hwf_e, hwf_cs, cs', S0, t0, hr, hwf_cs', hR0_sub, ?_⟩
-      intro m' denot hsub hproper himply hpure
+      intro m' denot hsub hproper himply_simple_ans himply hpure
       let R0 := expand_captures m.heap cs'
       have ih2 := rebind_exi_exp_denot (ρ.liftTVar (d:=denot)) T2 R0
       have himply' : denot.ImplyAfter m' (Ty.val_denot env1 T1) := by
         intro m'' hsub' e' hdenot
         exact (ih1 m'' e').mpr (himply m'' hsub' e' hdenot)
-      specialize hd m' denot hsub hproper himply' hpure
+      specialize hd m' denot hsub hproper himply_simple_ans himply' hpure
       exact (ih2 m' _).mp hd
     · intro ⟨hwf_e, hwf_cs, cs', S0, t0, hr, hwf_cs', hR0_sub, hd⟩
       refine ⟨hwf_e, hwf_cs, cs', S0, t0, hr, hwf_cs', hR0_sub, ?_⟩
-      intro m' denot hsub hproper himply hpure
+      intro m' denot hsub hproper himply_simple_ans himply hpure
       let R0 := expand_captures m.heap cs'
       have ih2 := rebind_exi_exp_denot (ρ.liftTVar (d:=denot)) T2 R0
       have himply' : denot.ImplyAfter m' (Ty.val_denot env2 (T1.rename f)) := by
         intro m'' hsub' e' hdenot
         exact (ih1 m'' e').mp (himply m'' hsub' e' hdenot)
-      specialize hd m' denot hsub hproper himply' hpure
+      specialize hd m' denot hsub hproper himply_simple_ans himply' hpure
       exact (ih2 m' _).mpr hd
   | .cpoly B cs T => by
     intro m e
